Test/civl/regression-tests/linear_types_error.bpl
@@ -7,57 +7,16 @@ atomic action {:layer 1, 2} A1(path: Lheap int) returns (path': Lheap int) {
     path' := path;
 }
 
-atomic action {:layer 1, 2} A2(path: Lheap int) returns (path': Lheap int) {
-    call path' := Lheap_Empty();
-    call Lheap_Put(path', path);
+atomic action {:layer 1, 2} A2(path: Lheap int) returns (path': Lheap int) { var k: Lset (Ref int);
+    call path' := Lmap_Empty();
+    call k := Lmap_Free(path);
 }
 
 var {:layer 0, 2} g: Lheap int;
 
-atomic action {:layer 1, 2} A3({:linear_in} path: Lheap int) returns (path': Lheap int)
-{
-    path' := path;
-    call Lheap_Put(path', g);
-}
-
 datatype Foo { Foo(f: Lheap int) }
 
-
-atomic action {:layer 1, 2} A4({:linear_in} path: Lheap Foo, x: Ref Foo, {:linear_in} l: Lheap int) returns (path': Lheap Foo, l': Lheap int)
-{
-    path' := path;
-    l' := l;
-    call Lheap_Put(l', path'->val[x]->f);
-}
-
 atomic action {:layer 1, 2} A5({:linear_out} path: Lheap int) { }
-
-atomic action {:layer 1, 2} A6({:linear_in} path: Lheap int) returns (path': Lheap int)
-{
-    path' := path;
-    call Lheap_Put(path', path');
-}
-
-atomic action {:layer 1, 2} A7(path1: Lheap int, {:linear_in} path2: Lheap int) returns (path': Lheap int)
-{
-    path' := path2;
-    call Lheap_Put(path', path1);
-}
-
-atomic action {:layer 1, 2} A8({:linear_in} path1: Lheap int, x: Ref Foo) returns (path2: Lheap Foo)
-{
-    call Lheap_Put(path2->val[x]->f, path1);
-}
-
-atomic action {:layer 1, 2} A9({:linear_in} l: Lheap int)
-{
-    call Lheap_Put(g, l);
-}
-
-atomic action {:layer 1, 2} A10({:linear_in} l: Lheap int, l': Lheap int)
-{
-    call Lheap_Put(l', l);
-}
 
 atomic action {:layer 1, 2} A11({:linear_in} a: Foo) returns (b: Foo)
 {
